theories/program_logic/infinite_traces.v
@@ -1,0 +1,189 @@
+From aneris.program_logic Require Export weakestpre traces.
+
+Set Default Proof Using "Type".
+
+Delimit Scope inflist_scope with inflist.
+
+CoInductive inflist (A : Type) : Type :=
+| infnil
+| infcons (x : A) (il : inflist A).
+
+Bind Scope inflist_scope with inflist.
+
+Arguments infnil {_}, _.
+Arguments infcons {_} _ _%inflist.
+
+Module InfListNotations.
+Notation "[ ]" := infnil (format "[ ]") : inflist_scope.
+Notation "[ x ]" := (infcons x infnil) : inflist_scope.
+Notation "[ x ; y ; .. ; z ]" :=
+  (infcons x (infcons y .. (infcons z nil) ..)) : inflist_scope.
+
+Infix "::" := infcons (at level 60, right associativity) : inflist_scope.
+End InfListNotations.
+
+Import InfListNotations.
+
+Section inflist.
+  Context {A : Type}.
+
+  Implicit Types il : inflist A.
+
+  Lemma inflist_unfold_fold il :
+    il = match il with
+         | [] => []
+         | a :: il' => a :: il'
+         end%inflist.
+  Proof. destruct il; trivial. Qed.
+
+End inflist.
+
+Definition inf_execution_trace Λ := inflist (list (observation Λ) * cfg Λ).
+
+Section inf_execution_trace.
+  Context {Λ : language}.
+
+  Definition inf_exec_prepend (κ : list (observation Λ)) (c : cfg Λ)
+             (iex : inf_execution_trace Λ) : inf_execution_trace Λ :=
+    ((κ, c) :: iex)%inflist.
+
+  CoInductive valid_inf_exec :
+    execution_trace Λ → inf_execution_trace Λ → Prop :=
+  | valid_inf_exec_singleton ex :
+      valid_exec ex → valid_inf_exec ex []%inflist
+  | valid_inf_exec_step ex c κ c' iex :
+      valid_exec ex →
+      exec_ends_in ex c →
+      step c κ c' →
+      valid_inf_exec (exec_extend ex κ c') iex →
+      valid_inf_exec ex (inf_exec_prepend κ c' iex).
+
+End inf_execution_trace.
+
+Definition inf_auxiliary_trace {Λ} (AS : AuxState Λ) := inflist (aux_state AS).
+
+Definition inf_auxtr_prepend `{AS : AuxState Λ}
+           (δ : aux_state AS) (atr : inf_auxiliary_trace AS) := infcons δ atr.
+
+CoInductive valid_inf_system_trace `{AS : AuxState Λ}
+            (Ψ : execution_trace Λ → auxiliary_trace AS → Prop) :
+  execution_trace Λ → auxiliary_trace AS →
+  inf_execution_trace Λ → inf_auxiliary_trace AS → Prop :=
+| valid_system_trace_singleton ex atr :
+    Ψ ex atr →
+    valid_inf_system_trace Ψ ex atr []%inflist []%inflist
+| valid_system_trace_step ex atr c κ c' δ δ' iex iatr :
+    Ψ ex atr →
+    exec_ends_in ex c →
+    step c κ c' →
+    auxtr_ends_in atr δ →
+    valid_state_evolution AS c.2 δ κ c'.2 δ' →
+    valid_inf_system_trace
+      Ψ (exec_extend ex κ c') (auxtr_extend atr δ') iex iatr →
+    valid_inf_system_trace
+      Ψ ex atr (inf_exec_prepend κ c' iex) (inf_auxtr_prepend δ' iatr).
+
+Section simulation.
+  Context {Λ : language} {AS : AuxState Λ}
+          {φ : execution_trace Λ → auxiliary_trace AS → Prop}.
+
+  Implicit Types ex : execution_trace Λ.
+  Implicit Types iex : inf_execution_trace Λ.
+
+  Lemma valid_inf_exec_prepend_valid_exec_extend ex κ c iex :
+    valid_inf_exec ex (inf_exec_prepend κ c iex) →
+    valid_exec (exec_extend ex κ c).
+  Proof.
+    inversion 1 as [|???????? Hex]; simplify_eq.
+    inversion Hex; done.
+  Qed.
+
+  Lemma produce_inf_aux_trace_next_aux_state_exists
+        (ex : execution_trace Λ) (atr : auxiliary_trace AS)
+        (Hcsm : continued_simulation φ ex atr)
+        (c : cfg Λ) (κ : list (observation Λ))
+        (iex : inf_execution_trace Λ)
+        (Hvex : valid_inf_exec ex (inf_exec_prepend κ c iex)) :
+    ∃ δ, continued_simulation φ (exec_extend ex κ c) (auxtr_extend atr δ).
+  Proof.
+    apply continued_simulation_next_aux_state_exists; first done.
+    eapply valid_inf_exec_prepend_valid_exec_extend; eauto.
+  Qed.
+
+  Definition produce_inf_aux_trace_next_aux_state
+             (ex : execution_trace Λ) (atr : auxiliary_trace AS)
+             (Hcsm : continued_simulation φ ex atr)
+             (c : cfg Λ) (κ : list (observation Λ))
+             (iex : inf_execution_trace Λ)
+             (Hvex : valid_inf_exec ex (inf_exec_prepend κ c iex))
+    : aux_state AS :=
+    epsilon
+      (produce_inf_aux_trace_next_aux_state_exists ex atr Hcsm c κ iex Hvex).
+
+  Lemma produce_inf_aux_trace_next_aux_state_continued_simulation
+        (ex : execution_trace Λ) (atr : auxiliary_trace AS)
+        (Hcsm : continued_simulation φ ex atr)
+        (c : cfg Λ) (κ : list (observation Λ))
+        (iex : inf_execution_trace Λ)
+        (Hvex : valid_inf_exec ex (inf_exec_prepend κ c iex)) :
+    continued_simulation
+      φ
+      (exec_extend ex κ c)
+      (auxtr_extend
+         atr (produce_inf_aux_trace_next_aux_state ex atr Hcsm c κ iex Hvex)).
+  Proof.
+    rewrite /produce_inf_aux_trace_next_aux_state.
+    apply epsilon_correct.
+  Qed.
+
+  Local Lemma valid_inf_exec_adjust {ex c κ iex} :
+    valid_inf_exec ex ((κ, c) :: iex)%inflist →
+    valid_inf_exec (exec_extend ex κ c) iex.
+  Proof. inversion 1; done. Qed.
+
+  CoFixpoint produce_inf_aux_trace
+          (ex : execution_trace Λ) (atr : auxiliary_trace AS)
+          (Hcsm : continued_simulation φ ex atr)
+          (iex : inf_execution_trace Λ)
+          (Hvex : valid_inf_exec ex iex) :
+    inf_auxiliary_trace AS :=
+    match iex as l return valid_inf_exec ex l → inf_auxiliary_trace AS with
+    | [] => λ _, []
+    | (κ, c) :: iex' =>
+      λ Hvex',
+      let δ :=
+          produce_inf_aux_trace_next_aux_state ex atr Hcsm c κ iex' Hvex'
+      in
+      δ :: (produce_inf_aux_trace
+              (exec_extend ex κ c)
+              (auxtr_extend atr δ)
+              (produce_inf_aux_trace_next_aux_state_continued_simulation
+                 ex atr Hcsm c κ iex' Hvex')
+              iex'
+              (valid_inf_exec_adjust Hvex'))
+    end%inflist Hvex.
+
+  Theorem produced_inf_aux_trace_valid_inf
+        (ex : execution_trace Λ) (atr : auxiliary_trace AS)
+        (Hcsm : continued_simulation φ ex atr)
+        (iex : inf_execution_trace Λ)
+        (Hvex : valid_inf_exec ex iex)
+    : valid_inf_system_trace
+        (continued_simulation φ)
+        ex atr
+        iex
+        (produce_inf_aux_trace ex atr Hcsm iex Hvex).
+  Proof.
+    revert ex atr Hcsm iex Hvex; cofix CIH; intros ex atr Hcsm iex Hvex.
+    destruct iex as [|[κ c] iex].
+    - rewrite [produce_inf_aux_trace _ _ _ _ _]inflist_unfold_fold /=.
+      constructor; trivial.
+    - rewrite [produce_inf_aux_trace _ _ _ _ _]inflist_unfold_fold /=.
+      pose proof (produce_inf_aux_trace_next_aux_state_continued_simulation
+                    ex atr Hcsm c κ iex Hvex) as Hcsm'.
+      pose proof (continued_simulation_valid_system_trace _ _ _ Hcsm') as Hvst.
+      apply valid_system_trace_extend_inv in Hvst as (?&?&?&?&?&?&?).
+      econstructor; eauto.
+  Qed.
+
+End simulation.
